tagless final Memoize instance

Validator/Regex/EnterMem.lean
@@ -6,22 +6,23 @@ import Validator.Regex.Regex
 
 namespace Regex
 
-def MemTable.enterM [DecidableEq σ] [Hashable σ] [Monad m] [MonadState (MemTable (@enter σ)) m]
+abbrev enterParam (σ: Type) := Regex σ
+abbrev enterMemTable (σ: Type) [DecidableEq σ] [Hashable σ] := MemTable enter (α := enterParam σ)
+abbrev enterResult (r: Regex σ) := IfExpr σ (symbols r)
+
+def MemTable.enterM [DecidableEq σ] [Hashable σ] [Monad m] [monadState: MonadState (enterMemTable σ) m]
   (param: Regex σ): m { res // res = enter param } :=
   MemTable.call enter param
 
-private theorem MemTable.enterM_is_correct [DecidableEq σ] [Hashable σ] (param: Regex σ) (table: (MemTable (@enter σ))):
+private theorem MemTable.enterM_is_correct [DecidableEq σ] [Hashable σ] (param: enterParam σ) (table: (enterMemTable σ)):
   enter param = (StateM.run (s := table) (MemTable.enterM param)).1 := by
   generalize (StateM.run (MemTable.enterM param) table) = x
   obtain ⟨⟨res, hres⟩, table'⟩ := x
   simp only
   rw [hres]
 
-abbrev enterParam (σ: Type) := Regex σ
-abbrev enterMemTable (σ: Type) [DecidableEq σ] [Hashable σ] := MemTable enter (α := enterParam σ)
-
-instance [DecidableEq σ] [Hashable σ] [Monad m] [MonadState (MemTable (@enter σ)) m]:
-  Memoize (α := Regex σ) (β := fun r => IfExpr σ (symbols r)) enter m where
+instance [DecidableEq σ] [Hashable σ] [Monad m] [MonadState (enterMemTable σ) m]:
+  Memoize (α := enterParam σ) (β := enterResult) enter m where
   call param := MemTable.enterM param
 
 abbrev MemoizedEnter (σ: Type) [DecidableEq σ] [Hashable σ] := Memoize (@enter σ) (StateM (enterMemTable σ))
