Validator/Regex/LeaveMem.lean
@@ -6,25 +6,27 @@ import Validator.Regex.Leave
 
 namespace Regex
 
-def leave2 {σ: Type}: (Σ (r: Regex σ), (Vector Bool (symbols r))) → Regex σ
+abbrev leaveParam (σ: Type) := Σ (r: Regex σ), (Vector Bool (symbols r))
+abbrev leaveResult {σ: Type} (_: leaveParam σ) := Regex σ
+
+def leave2 {σ: Type}: (a: leaveParam σ) → leaveResult a
   | ⟨r, bools⟩ => leave r bools
 
-def MemTable.leaveM {σ: Type} [DecidableEq σ] [Hashable σ] [Monad m] [MonadState (MemTable leave2 (α := (Σ (r: Regex σ), (Vector Bool (symbols r))))) m]
-  (param: Σ (r: Regex σ), (Vector Bool (symbols r))): m { res // res = leave2 param } :=
+abbrev leaveMemTable (σ: Type) [DecidableEq σ] [Hashable σ] := MemTable leave2 (α := leaveParam σ)
+
+def MemTable.leaveM {σ: Type} [DecidableEq σ] [Hashable σ] [Monad m] [monadState: MonadState (leaveMemTable σ) m]
+  (param: leaveParam σ): m { res // res = leave2 param } :=
   MemTable.call leave2 param
 
-private theorem MemTable.leaveM_is_correct [DecidableEq σ] [Hashable σ] (param: Σ (r: Regex σ), (Vector Bool (symbols r))) (table: (MemTable (@leave2 σ))):
+private theorem MemTable.leaveM_is_correct [DecidableEq σ] [Hashable σ] (param: leaveParam σ) (table: leaveMemTable σ):
   leave2 param = (StateM.run (s := table) (leaveM param)).1 := by
   generalize (StateM.run (leaveM param) table) = x
   obtain ⟨⟨res, hres⟩, table'⟩ := x
   simp only
   rw [hres]
 
-abbrev leaveParam (σ: Type) := Σ (r: Regex σ), (Vector Bool (symbols r))
-abbrev leaveMemTable (σ: Type) [DecidableEq σ] [Hashable σ] := MemTable leave2 (α := leaveParam σ)
-
 instance {σ: Type} [DecidableEq σ] [Hashable σ] [Monad m] [MonadState (leaveMemTable σ) m]:
-  Memoize (α := leaveParam σ) (β := fun _ => Regex σ) leave2 m where
+  Memoize (α := leaveParam σ) (β := leaveResult) leave2 m where
   call param := MemTable.leaveM param
 
 abbrev MemoizedLeave (σ: Type) [DecidableEq σ] [Hashable σ] := Memoize (@leave2 σ) (StateM (leaveMemTable σ))
