Validator/Regex/Memoize.lean
@@ -6,13 +6,33 @@ import Validator.Regex.Drawer
 import Validator.Regex.IfExpr
 import Validator.Regex.Lang
 import Validator.Regex.Leave
+import Validator.Regex.LeaveMem
 import Validator.Regex.Num
 import Validator.Regex.Regex
 
-def Regex.Mem.derive
-  [DecidableEq σ] [Hashable σ]
-  [mementer: MemoizedEnter σ]
-  (Φ: σ → Bool) (r: Regex σ): StateM (MemTable (@enter σ)) (Regex σ) := do
-  let ⟨ifexpr, _⟩ <- mementer.call r
-  let bools := IfExpr.eval Φ ifexpr
-  return leave r bools
+namespace Regex
+
+-- class Memoize {α: Type} [DecidableEq α] [Hashable α] {β: α -> Type} (f: (a: α) → β a) (m: Type -> Type u) where
+--   call : (a: α) -> m { b: β a // b = f a }
+
+class MemoizeRoom (m: Type -> Type u) (σ: Type) [DecidableEq σ] [Hashable σ] where
+  enterM : (a: enterParam σ) -> m { b: enterResult a // b = enter a }
+  leaveM : (a: leaveParam σ) -> m { b: leaveResult a // b = leave2 a }
+
+instance (m: Type -> Type u) (σ: Type) [DecidableEq σ] [Hashable σ] [Monad m]
+  [DecidableEq (enterParam σ)] [Hashable (enterParam σ)]
+  [Memoize (α := enterParam σ) (β := enterResult) enter m]
+  [enterState: MonadState (enterMemTable σ) m]
+  [DecidableEq (leaveParam σ)] [Hashable (leaveParam σ)]
+  [Memoize (α := leaveParam σ) (β := leaveResult) leave2 m]
+  [leaveState: MonadState (leaveMemTable σ) m]
+  : MemoizeRoom m σ where
+  enterM param := MemTable.enterM (monadState := enterState) param
+  leaveM param := MemTable.leaveM (monadState := leaveState) param
+
+end Regex
+
+def Regex.Mem.derive [Monad m] [DecidableEq σ] [Hashable σ] [MemoizeRoom m σ]
+  (Φ: σ → Bool) (r: Regex σ): m (Regex σ) := do
+  let ifexpr <- MemoizeRoom.enterM r
+  MemoizeRoom.leaveM ⟨r, IfExpr.eval Φ ifexpr⟩
